coq/soundness.v
@@ -1,0 +1,7 @@
+Require Export lc.tactics.
+Require Export lc.relations.
+Require Import Lia.
+Require Import Coq.Logic.FunctionalExtensionality.
+
+Import LCNotations.
+Local Open Scope lc_scope.
